tests/lean/run/type_equations.lean
@@ -1,0 +1,38 @@
+open nat
+
+inductive expr :=
+| zero : expr
+| one  : expr
+| add  : expr → expr → expr
+
+namespace expr
+
+inductive direct_subterm : expr → expr → Prop :=
+| add_1 : ∀ e₁ e₂ : expr, direct_subterm e₁ (add e₁ e₂)
+| add_2 : ∀ e₁ e₂ : expr, direct_subterm e₂ (add e₁ e₂)
+
+theorem direct_subterm_wf : well_founded direct_subterm :=
+begin
+  constructor, intro e, induction e,
+  repeat (constructor; intro y hlt; cases hlt; repeat assumption)
+end
+
+definition subterm := tc direct_subterm
+
+theorem subterm_wf [instance] : well_founded subterm :=
+tc.wf direct_subterm_wf
+
+infix `+` := expr.add
+
+set_option pp.notation false
+
+definition ev : expr → nat
+| zero             := 0
+| one              := 1
+| ((a : expr) + b) := ev a + ev b
+
+definition foo : expr := add zero (add one one)
+
+example : ev foo = 2 :=
+rfl
+end expr
